end of day 26/07/18

michael_formal/EFSM.thy
@@ -2,6 +2,10 @@ theory EFSM
   imports Types
 begin
 
+definition
+  S :: "'statename efsm \<Rightarrow> 'statename set" where
+  "S m = {a. (\<exists>x. (T m) (a, x) \<noteq> {}) \<or> (\<exists>x. (T m) (x, a) \<noteq> {})}"
+
 primrec apply_outputs :: "output_function list \<Rightarrow> datastate \<Rightarrow> outputs" where
   "apply_outputs [] _ = []" |
   "apply_outputs (h#t) s = (case aval h s of None \<Rightarrow> [] | Some p \<Rightarrow> p#(apply_outputs t s))"
@@ -18,19 +22,18 @@ lemma "apply_updates [(R 1, L (Num 6))] <> <R 2:= Num 3> = <R 1:= Num 6, R 2:= N
   apply (rule ext)
   by simp
 
-abbreviation is_possible_step :: "efsm \<Rightarrow> statename \<Rightarrow> statename \<Rightarrow> transition \<Rightarrow> datastate \<Rightarrow> label \<Rightarrow> inputs \<Rightarrow> bool" where
-"is_possible_step e s s' t r l i \<equiv> (((Label t) = l) \<and> (find (\<lambda>x . x = t) (T e(s,s')) \<noteq> None) \<and> ((length i) = (Arity t)) \<and> (apply_guards (Guard t) (join_ir i r)))"
+abbreviation is_possible_step :: "'statename efsm \<Rightarrow> 'statename \<Rightarrow> 'statename \<Rightarrow> transition \<Rightarrow> datastate \<Rightarrow> label \<Rightarrow> inputs \<Rightarrow> bool" where
+"is_possible_step e s s' t r l i \<equiv> (((Label t) = l) \<and> (t \<in> T e (s,s')) \<and> ((length i) = (Arity t)) \<and> (apply_guards (Guard t) (join_ir i r)))"
 
-abbreviation possible_steps :: "efsm \<Rightarrow> statename \<Rightarrow> datastate \<Rightarrow> label \<Rightarrow> inputs \<Rightarrow> (statename * transition) list" where
-"possible_steps e s r l i \<equiv> [(s',t) . s' \<leftarrow> S e, t \<leftarrow> T e(s,s'), is_possible_step e s s' t r l i]"
+definition possible_steps :: "'statename efsm \<Rightarrow> 'statename \<Rightarrow> datastate \<Rightarrow> label \<Rightarrow> inputs \<Rightarrow> ('statename \<times> transition) set" where
+(* "possible_steps e s r l i \<equiv> {(s',t) . s' \<in> S e \<and> t \<in> T e (s,s') \<and> is_possible_step e s s' t r l i}" *)
+"possible_steps e s r l i \<equiv> {(s',t). is_possible_step e s s' t r l i}"
 
-definition step :: "efsm \<Rightarrow> statename \<Rightarrow> datastate \<Rightarrow> label \<Rightarrow> inputs \<Rightarrow> (statename \<times> outputs \<times> datastate) option" where
+abbreviation step :: "'statename efsm \<Rightarrow> 'statename \<Rightarrow> datastate \<Rightarrow> label \<Rightarrow> inputs \<Rightarrow> ('statename \<times> outputs \<times> datastate) option" where
 "step e s r l i \<equiv>
-  case (possible_steps e s r l i) of
-    [(s',t)] \<Rightarrow> Some (s', (apply_outputs (Outputs t) (join_ir i r)), (apply_updates (Updates t) (join_ir i r) r)) |
-    _ \<Rightarrow> None"
+(if is_singleton (possible_steps e s r l i) then (let (s', t) =  (the_elem (possible_steps e s r l i)) in Some (s', (apply_outputs (Outputs t) (join_ir i r)), (apply_updates (Updates t) (join_ir i r) r))) else None)"
 
-primrec observe_temp :: "efsm \<Rightarrow> statename \<Rightarrow> datastate \<Rightarrow> trace \<Rightarrow> (statename \<times> event \<times> datastate \<times> outputs) list" where
+primrec observe_temp :: "'statename efsm \<Rightarrow> 'statename \<Rightarrow> datastate \<Rightarrow> trace \<Rightarrow> ('statename \<times> event \<times> datastate \<times> outputs) list" where
   "observe_temp e s r [] = []" |
   "observe_temp e s r (h#t) =
     (case (step e s r (fst h) (snd h)) of
@@ -38,7 +41,7 @@ primrec observe_temp :: "efsm \<Rightarrow> statename \<Rightarrow> datastate \<
       _ \<Rightarrow> []
     )"
 
-primrec observe_all :: "efsm \<Rightarrow> statename \<Rightarrow> datastate \<Rightarrow> trace \<Rightarrow> (statename \<times> outputs \<times> datastate) list" where
+primrec observe_all :: "'statename efsm \<Rightarrow> 'statename \<Rightarrow> datastate \<Rightarrow> trace \<Rightarrow> ('statename \<times> outputs \<times> datastate) list" where
   "observe_all _ _ _ [] = []" |
   "observe_all e s r (h#t) = 
     (case (step e s r (fst h) (snd h)) of
@@ -46,10 +49,10 @@ primrec observe_all :: "efsm \<Rightarrow> statename \<Rightarrow> datastate \<R
       _ \<Rightarrow> []
     )"
 
-abbreviation observe_trace :: "efsm \<Rightarrow> statename \<Rightarrow> datastate \<Rightarrow> trace \<Rightarrow> observation" where
+abbreviation observe_trace :: "'statename efsm \<Rightarrow> 'statename \<Rightarrow> datastate \<Rightarrow> trace \<Rightarrow> observation" where
   "observe_trace e s r t \<equiv> map (\<lambda>(x,y,z). y) (observe_all e s r t)"
 
-definition equiv :: "efsm \<Rightarrow> efsm \<Rightarrow> trace \<Rightarrow> bool" where
+definition equiv :: "'statename efsm \<Rightarrow> 'statename efsm \<Rightarrow> trace \<Rightarrow> bool" where
   "equiv e1 e2 t \<equiv> ((observe_trace e1 (s0 e1) <> t) = (observe_trace e2 (s0 e2) <> t))"
 
 lemma equiv_comute: "equiv e1 e2 t \<equiv> equiv e2 e1 t"
@@ -62,7 +65,7 @@ lemma equiv_trans: "equiv e1 e2 t \<and> equiv e2 e3 t \<longrightarrow> equiv e
 lemma equiv_idem: "equiv e1 e1 t"
   by (simp add: equiv_def)
 
-abbreviation valid_trace :: "efsm \<Rightarrow> trace \<Rightarrow> bool" where
+abbreviation valid_trace :: "'statename efsm \<Rightarrow> trace \<Rightarrow> bool" where
   "valid_trace e t \<equiv> (length t = length (observe_all e (s0 e) <> t))"
 
 lemma empty_trace_valid [simp]: "valid_trace e []"
@@ -72,9 +75,6 @@ primrec in_list :: "'a \<Rightarrow> 'a list \<Rightarrow> bool" where
   "in_list _ [] = False" |
   "in_list x (h#t) = (if (x=h) then True else (in_list x t))"
 
-definition all_outs :: "efsm \<Rightarrow> statename \<Rightarrow> destination list" where
-  "all_outs e s = [(s',t) . s' \<leftarrow> S e, t \<leftarrow> T e(s,s'), (in_list t (T e(s,s')))]"
-
 definition can_take :: "transition \<Rightarrow> transition \<Rightarrow> bool" where
   "can_take t1 t2 \<equiv> ((Label t1) = (Label t2)) \<and> ((Arity t1) = (Arity t2))"
 
@@ -83,7 +83,8 @@ primrec find_match :: "transition \<Rightarrow> destination list \<Rightarrow> d
   "find_match t (h#tail) = (if (can_take t (snd h)) then (Some h) else (find_match t tail))"
 
 lemma valid_unit_trace: "step e (s0 e) <> l i = Some (s',outs,r) \<Longrightarrow> valid_trace e [(l,i)]"
-  by auto
+  apply (simp add: is_singleton_def the_elem_def possible_steps_def)
+  using Suc_length_conv by fastforce
 
 lemma different_observation_techniques: 
   shows "length(observe_all e s r t) = length(observe_trace e s r t)"
