michael_formal/EFSM_LTL.thy
@@ -27,4 +27,35 @@ fun ltl_step :: "efsm \<Rightarrow> statename option \<Rightarrow> datastate \<R
 primcorec make_full_observation :: "efsm \<Rightarrow> statename option \<Rightarrow> datastate \<Rightarrow> event stream \<Rightarrow> full_observation" where
   "make_full_observation e s d i = (let (s', o', d') = ltl_step e s d (shd i) in \<lparr>statename = s, datastate = d, event=(shd i), output = o'\<rparr>##(make_full_observation e s' d' (stl i)))"
 
+abbreviation non_null :: property where
+  "non_null s \<equiv> (statename (shd s) \<noteq> None)"
+
+abbreviation null :: property where
+  "null s \<equiv> (statename (shd s) = None)"
+
+lemma null_forever [simp]: "s = make_full_observation e (Some (s0 e)) <> t \<Longrightarrow> null s \<Longrightarrow> nxt (alw null) s"
+  by simp
+
+abbreviation some_state :: "full_observation \<Rightarrow> bool" where
+  "some_state s \<equiv> (\<exists>state. statename (shd s) = Some state)"
+
+lemma non_null_equiv: "non_null = some_state"
+  by simp
+
+lemma start_some_state:  "s = make_full_observation e (Some (s0 e)) <> t \<Longrightarrow> some_state s"
+  by simp
+
+lemma self_eq:  "make_full_observation e (Some (s0 e)) <> t = make_full_observation e (Some (s0 e)) <> t"
+  by simp
+
+
+lemma some_until_none: "s = make_full_observation e (Some (s0 e)) <> t \<Longrightarrow> (some_state until null) s "
+proof (coinduction)
+  case UNTIL
+  then show ?case
+    by (smt UNTIL.coinduct non_null_equiv)
+qed
+
+
+
 end
