michael_formal/drinks_machine.thy
@@ -5,6 +5,8 @@ begin
 (* This version of drinks_machine supercedes all of those before 03/04/18 *)
 (* It also supercedes "drinks.thy"*)
 
+datatype statename = q1 | q2 | q3
+
 definition select :: "transition" where
 "select \<equiv> \<lparr>
         Label = ''select'',
@@ -18,6 +20,9 @@ definition select :: "transition" where
       \<rparr>"
 
 lemma guard_select [simp]: "Guard select = []"
+  by (simp add: select_def)
+
+lemma outputs_select [simp]: "Outputs select = []"
   by (simp add: select_def)
 
 definition coin :: "transition" where
@@ -44,45 +49,130 @@ definition vend :: "transition" where
         Updates = [(R 1, V (R 1)), (R 2, V (R 2))]
       \<rparr>"
 
-definition drinks :: "efsm" where
+definition drinks :: "statename efsm" where
 "drinks \<equiv> \<lparr> 
-          S = [1,2,3],
-          s0 = 1,
+          s0 = q1,
           T = \<lambda> (a,b) .
-              if (a,b) = (1,2) then [select] (* If we want to go from state 1 to state 2 then select will do that *)
-              else if (a,b) = (2,2) then [coin] (* If we want to go from state 2 to state 2 then coin will do that *)
-              else if (a,b) = (2,3) then [vend] (* If we want to go from state 2 to state 3 then vend will do that *)
-              else [] (* There are no other transitions *)
+              if (a,b) = (q1,q2) then {select} (* If we want to go from state 1 to state 2 then select will do that *)
+              else if (a,b) = (q2,q2) then {coin} (* If we want to go from state 2 to state 2 then coin will do that *)
+              else if (a,b) = (q2,q3) then {vend} (* If we want to go from state 2 to state 3 then vend will do that *)
+              else {} (* There are no other transitions *)
          \<rparr>"
+
+lemma s0_drinks [simp]: "s0 drinks = q1"
+  by (simp add: drinks_def)
 
 (*
   These are lemmas about the machine which could maybe be in another file.
   They don't need to be translated to SAL
 *)
 
-lemmas transitions = select_def coin_def vend_def
+lemmas transitions = select_def coin_def vend_def is_singleton_def the_elem_def
 
 lemma "observe_trace drinks (s0 drinks) <> [] = []"
   by simp
 
+lemma label_select_q2: "Label t = ''select'' \<and>
+             t \<in> (if s' = q2 then {select} else if (q1, s') = (q2, q2) then {coin} else if (q1, s') = (q2, q3) then {vend} else {}) \<Longrightarrow> t = select \<and> s' = q2"
+  apply (cases s')
+    apply simp
+   apply simp
+  by (simp add: select_def)
+
+lemma label_coin_q2: "Label b = ''coin'' \<Longrightarrow>
+           b \<in> (if a = q2 then {coin} else if (q2, a) = (q2, q3) then {vend} else {}) \<Longrightarrow> b=coin \<and> a = q2"
+  apply (cases a)
+    apply simp
+   apply simp
+  by (simp add: vend_def)
+
+lemma label_vend_q3: "Label b = ''vend'' \<Longrightarrow>
+           b \<in> (if a = q2 then {coin} else if (q2, a) = (q2, q3) then {vend} else {}) \<Longrightarrow> b=vend \<and> a = q3"
+  apply (cases a)
+    apply simp
+   apply (simp add: coin_def)
+  by (simp add: vend_def)
+
+lemma possible_steps_q1:  "possible_steps drinks q1 Map.empty ''select'' [Str ''coke''] = {(q2, select)}"
+  apply (simp add: possible_steps_def drinks_def)
+  apply safe
+       apply (meson empty_iff old.prod.inject statename.distinct(1))
+      apply (meson empty_iff old.prod.inject singletonD statename.distinct(1))
+  by (simp_all add: select_def)
+
 lemma "observe_trace drinks (s0 drinks) <> [(''select'', [Str ''coke''])] = [[]]"
-  by (simp add: drinks_def transitions step_def)
+  by (simp add: is_singleton_def the_elem_def possible_steps_q1)
+
+lemma select_updates [simp]: "(apply_updates (Updates select) (case_vname (\<lambda>n. if n = Suc 0 then Some (Str ''coke'') else index2state [] (Suc 0 + 1) (I n)) Map.empty) Map.empty) = <R 1:=Str ''coke'', R 2 := Num 0>"
+  apply (simp add: select_def)
+  apply (rule ext)
+  by simp
+
+lemma possible_steps_q2_coin: "possible_steps drinks q2 <R (Suc 0) := Str ''coke'', R 2 := Num 0> ''coin'' [Num 50] = {(q2, coin)}"
+  apply (simp add: possible_steps_def drinks_def)
+  apply safe
+  using label_coin_q2 apply blast
+      apply (metis One_nat_def empty_iff one_neq_zero singletonD transition.select_convs(2) vend_def)
+  by (simp_all add: coin_def)
+
+lemma possible_steps_q2_coin_2: "possible_steps drinks q2 <R (Suc 0) := Str ''coke'', R 2 := Num 50> ''coin'' [Num 50] = {(q2, coin)}"
+  apply (simp add: possible_steps_def drinks_def)
+  apply safe
+  using label_coin_q2 apply blast
+      apply (metis One_nat_def empty_iff one_neq_zero singletonD transition.select_convs(2) vend_def)
+  by (simp_all add: coin_def)
 
 lemma "observe_trace drinks (s0 drinks) <> [(''select'', [Str ''coke'']), (''coin'', [Num 50])] = [[], [Num 50]]"
-  by (simp_all add: step_def drinks_def transitions)
+  apply (simp add: is_singleton_def the_elem_def possible_steps_q1 possible_steps_q2_coin possible_steps_q2_coin_2)
+  by (simp add: coin_def)
+
+lemma coin_50_updates [simp]: "(apply_updates (Updates coin)
+               (case_vname (\<lambda>n. if n = Suc 0 then Some (Num 50) else index2state [] (Suc 0 + 1) (I n)) (\<lambda>n. if n = 2 then Some (Num 0) else <R (Suc 0) := Str ''coke''> (R n)))
+               <R (Suc 0) := Str ''coke'', R 2 := Num 0>) = <R 1 := Str ''coke'', R 2 := Num 50>"
+  apply (simp add: transitions)
+  apply (rule ext)
+  by simp
 
 lemma "observe_trace drinks (s0 drinks) <> [(''select'', [Str ''coke'']), (''coin'', [Num 50]), (''coin'', [Num 50])] = [[], [Num 50], [Num 100]]"
-  by (simp add: step_def drinks_def transitions)
+  apply (simp add: is_singleton_def the_elem_def possible_steps_q1 possible_steps_q2_coin possible_steps_q2_coin_2)
+  by (simp add: transitions)
+
+lemma coin_100_updates [simp]: "(apply_updates (Updates coin)
+               (case_vname (\<lambda>n. if n = Suc 0 then Some (Num 50) else index2state [] (Suc 0 + 1) (I n)) (\<lambda>n. if n = 2 then Some (Num 50) else <R (Suc 0) := Str ''coke''> (R n)))
+               <R (Suc 0) := Str ''coke'', R 2 := Num 50>) = <R 1 := Str ''coke'', R 2 := Num 100>"
+  apply (simp add: transitions)
+  apply (rule ext)
+  by simp
+
+lemma "possible_steps drinks q2 <R (Suc 0) := Str ''coke'', R 2 := Num 100> ''vend'' [] = {(q3, vend)}"
+  apply (simp add: possible_steps_def drinks_def)
+  apply safe
+       apply (metis coin_def empty_iff old.prod.inject one_neq_zero singletonD transition.select_convs(2))
+      apply (metis coin_def empty_iff one_neq_zero singleton_iff transition.select_convs(2))
+  by (simp_all add: vend_def)
 
 lemma "observe_trace drinks (s0 drinks) <> [(''select'', [Str ''coke'']), (''coin'', [Num 50]), (''coin'', [Num 50]), (''vend'', [])] = [[], [Num 50], [Num 100], [Str ''coke'']]"
-  by (simp add: step_def drinks_def transitions)
+  apply (simp add: is_singleton_def the_elem_def possible_steps_q1 possible_steps_q2_coin possible_steps_q2_coin_2)
+  by (simp add: transitions)
+
+lemma label_not_cat: "Label t = ''cat'' \<and>
+                       t \<in> T drinks (q2, s') \<Longrightarrow> False"
+  apply (simp add: drinks_def transitions)
+  apply (cases s')
+    apply simp
+   apply (simp add: coin_def)
+   apply auto[1]
+  apply (simp add: vend_def)
+  by auto
 
 (*Stop when we hit a spurious input*)
 lemma "observe_trace drinks (s0 drinks) <> [(''select'', [Str ''coke'']), (''cat'', [Num 50])] = [[]]"
-  by (simp add: step_def drinks_def transitions)
+  apply (simp add: is_singleton_def the_elem_def)
+  using label_not_cat by fastforce
 
 lemma "\<not> (valid_trace (drinks) [(''select'', [Str ''coke'']), (''cat'', [Num 50])])"
-  by(simp add: step_def drinks_def transitions)
+  apply (simp add: is_singleton_def the_elem_def drinks_def del: possible_steps.simps)
+
 
 lemma "observe_trace drinks (s0 drinks) <> [(''select'', [Str ''coke'']), (''cat'', [Num 50]), (''coin'', [Num 50])] = [[]]"
   by (simp add: step_def drinks_def transitions)
